code/k256/Hacl.K256.PrecompTable.fst
@@ -22,64 +22,22 @@ include Hacl.Impl.K256.Group
 
 #set-options "--z3rlimit 50 --fuel 0 --ifuel 0"
 
-inline_for_extraction noextract
-val proj_point_to_list: p:S.proj_point
-  -> x:list uint64{FStar.List.Tot.length x = 15 /\
-    mk_to_k256_comm_monoid.BE.linv (Seq.seq_of_list x)}
-
 let proj_point_to_list p =
   Hacl.Spec.K256.PrecompTable.proj_point_to_list_lemma p;
   Hacl.Spec.K256.PrecompTable.proj_point_to_list p
-
-
-val lemma_refl: x:S.proj_point ->
-  Lemma (S.mk_k256_concrete_ops.SE.to.SE.refl x ==
-    mk_to_k256_comm_monoid.BE.refl (Seq.seq_of_list (proj_point_to_list x)))
 
 let lemma_refl x =
   Hacl.Spec.K256.PrecompTable.proj_point_to_list_lemma x
 
 
-inline_for_extraction noextract
-let mk_k256_precomp_base_table: SPT.mk_precomp_base_table S.proj_point U64 15ul 0ul = {
-  SPT.concr_ops = S.mk_k256_concrete_ops;
-  SPT.to_cm = mk_to_k256_comm_monoid;
-  SPT.to_list = proj_point_to_list;
-  SPT.lemma_refl = lemma_refl;
-}
-
-
-inline_for_extraction noextract
-let pow_base_point (k:nat) =
-  LE.pow S.mk_k256_comm_monoid (S.to_aff_point S.g) k
-
-
-unfold
-let precomp_table_acc_inv
-  (table_len:nat{table_len * 15 <= max_size_t})
-  (table:LSeq.lseq uint64 (table_len * 15))
-  (j:nat{j < table_len})
-=
-  Math.Lemmas.lemma_mult_lt_right 15 j table_len;
-  Math.Lemmas.lemma_mult_le_right 15 (j + 1) table_len;
-  let bj = LSeq.sub table (j * 15) 15 in
-  point_inv_lseq bj /\ S.to_aff_point (point_eval_lseq bj) == pow_base_point j
-
-
-///  window size = 4
-
-unfold let precomp_basepoint_table_list_w4: x:list uint64{FStar.List.Tot.length x = 240} =
+let precomp_basepoint_table_list_w4: x:list uint64{FStar.List.Tot.length x = 240} =
   normalize_term (SPT.precomp_base_table_list mk_k256_precomp_base_table S.g 15)
 
 
-inline_for_extraction noextract
 let precomp_basepoint_table_lseq_w4 : LSeq.lseq uint64 240 =
   normalize_term_spec (SPT.precomp_base_table_list mk_k256_precomp_base_table S.g 15);
   Seq.seq_of_list precomp_basepoint_table_list_w4
 
-
-val precomp_basepoint_table_lemma_w4: unit ->
-  Lemma (forall (i:nat{i < 16}). precomp_table_acc_inv 16 precomp_basepoint_table_lseq_w4 i)
 
 let precomp_basepoint_table_lemma_w4 () =
   normalize_term_spec (SPT.precomp_base_table_list mk_k256_precomp_base_table S.g 15);
@@ -89,29 +47,3 @@ let precomp_basepoint_table_lemma_w4 () =
 let precomp_basepoint_table_w4:
   x:glbuffer uint64 240ul{witnessed x precomp_basepoint_table_lseq_w4 /\ recallable x} =
   createL_global precomp_basepoint_table_list_w4
-
-(*
-///  window size = 5
-
-unfold let precomp_basepoint_table_list_w5: x:list uint64{FStar.List.Tot.length x = 480} =
-  normalize_term (SPT.precomp_base_table_list mk_k256_precomp_base_table S.g 31)
-
-
-inline_for_extraction noextract
-let precomp_basepoint_table_lseq_w5 : LSeq.lseq uint64 480 =
-  normalize_term_spec (SPT.precomp_base_table_list mk_k256_precomp_base_table S.g 31);
-  Seq.seq_of_list precomp_basepoint_table_list_w5
-
-
-val precomp_basepoint_table_lemma_w5: unit ->
-  Lemma (forall (i:nat{i < 32}). precomp_table_acc_inv 32 precomp_basepoint_table_lseq_w5 i)
-
-let precomp_basepoint_table_lemma_w5 () =
-  normalize_term_spec (SPT.precomp_base_table_list mk_k256_precomp_base_table S.g 31);
-  SPT.precomp_base_table_lemma mk_k256_precomp_base_table S.g 32 precomp_basepoint_table_lseq_w5
-
-
-let precomp_basepoint_table_w5:
-  x:glbuffer uint64 480ul{witnessed x precomp_basepoint_table_lseq_w5 /\ recallable x} =
-  createL_global precomp_basepoint_table_list_w5
-*)
