code/k256/Hacl.K256.PrecompTable.fsti
@@ -1,0 +1,73 @@
+module Hacl.K256.PrecompTable
+
+open FStar.HyperStack
+open FStar.HyperStack.ST
+open FStar.Mul
+
+open Lib.IntTypes
+open Lib.Buffer
+
+module ST = FStar.HyperStack.ST
+module LSeq = Lib.Sequence
+
+module LE = Lib.Exponentiation
+module SE = Spec.Exponentiation
+module BE = Hacl.Impl.Exponentiation.Definitions
+module SPT = Hacl.Spec.PrecompBaseTable
+
+module S = Spec.K256
+
+open Hacl.Impl.K256.Point
+include Hacl.Impl.K256.Group
+
+#set-options "--z3rlimit 50 --fuel 0 --ifuel 0"
+
+inline_for_extraction noextract
+val proj_point_to_list: p:S.proj_point
+  -> x:list uint64{FStar.List.Tot.length x = 15 /\
+    mk_to_k256_comm_monoid.BE.linv (Seq.seq_of_list x)}
+
+val lemma_refl: x:S.proj_point ->
+  Lemma (S.mk_k256_concrete_ops.SE.to.SE.refl x ==
+    mk_to_k256_comm_monoid.BE.refl (Seq.seq_of_list (proj_point_to_list x)))
+
+
+inline_for_extraction noextract
+let mk_k256_precomp_base_table: SPT.mk_precomp_base_table S.proj_point U64 15ul 0ul = {
+  SPT.concr_ops = S.mk_k256_concrete_ops;
+  SPT.to_cm = mk_to_k256_comm_monoid;
+  SPT.to_list = proj_point_to_list;
+  SPT.lemma_refl = lemma_refl;
+}
+
+
+inline_for_extraction noextract
+let pow_base_point (k:nat) =
+  LE.pow S.mk_k256_comm_monoid (S.to_aff_point S.g) k
+
+
+unfold
+let precomp_table_acc_inv
+  (table_len:nat{table_len * 15 <= max_size_t})
+  (table:LSeq.lseq uint64 (table_len * 15))
+  (j:nat{j < table_len})
+=
+  Math.Lemmas.lemma_mult_lt_right 15 j table_len;
+  Math.Lemmas.lemma_mult_le_right 15 (j + 1) table_len;
+  let bj = LSeq.sub table (j * 15) 15 in
+  point_inv_lseq bj /\ S.to_aff_point (point_eval_lseq bj) == pow_base_point j
+
+
+///  window size = 4
+
+inline_for_extraction noextract
+val precomp_basepoint_table_list_w4: x:list uint64{FStar.List.Tot.length x = 240}
+
+inline_for_extraction noextract
+val precomp_basepoint_table_lseq_w4 : LSeq.lseq uint64 240
+
+val precomp_basepoint_table_lemma_w4: unit ->
+  Lemma (forall (i:nat{i < 16}). precomp_table_acc_inv 16 precomp_basepoint_table_lseq_w4 i)
+
+val precomp_basepoint_table_w4:
+  x:glbuffer uint64 240ul{witnessed x precomp_basepoint_table_lseq_w4 /\ recallable x}
